coq: Logic: Fol2: Proof

coq/Logic/Fol2/Axiom.v
@@ -1,5 +1,15 @@
+Require Import Logic.Class.Eq.
+
+Require Import Logic.Fol.Free.
 Require Import Logic.Fol.Syntax.
 
 (* Predicate determining whether a proposition is a set theoretic axiom         *)
 (* This is just a stub for now, no set theoretic axiom is defined for now       *)
-Definition IsAxiom (v:Type) (p:P v) : Prop := False.
+Definition IsAxiom (v:Type) (e:Eq v) (p:P v) : Prop := False.
+
+Arguments IsAxiom {v} {e}.
+
+Lemma axiomsClosed : forall (v:Type) (e:Eq v) (p:P v), IsAxiom p -> Fr p = nil.
+Proof.
+  intros v e p HAx. contradiction.
+Qed.
