coq/Logic/Fol2/Proof.v
@@ -1,16 +1,48 @@
+Require Import Logic.Class.Eq.
+
+Require Import Logic.Func.Permute.
+
+Require Import Logic.List.In.
+Require Import Logic.List.Include.
+
+
+Require Import Logic.Fol.Free.
+Require Import Logic.Fol.Functor.
 Require Import Logic.Fol.Syntax.
+
 Require Import Logic.Fol2.Context.
 Require Import Logic.Fol2.Axiom.
 
 Declare Scope Fol2_Proof_scope.
 
-Inductive Seq (v:Type) : Ctx v -> P v -> Type :=
-| Extract:forall (G:Ctx v)(p:P v),     Seq v (G;p) p 
-| WeakenP:forall (G:Ctx v)(p q:P v),   Seq v G p -> Seq v (G;q) p
-| WeakenV:forall (G:Ctx v)(x:v)(p:P v),Seq v G p -> Seq v (G,x) p
-| Deduct: forall (G:Ctx v)(p q:P v),   Seq v (G;p) q -> Seq v G (p :-> q)
-| Modus:  forall (G:Ctx v)(p q: P v),  Seq v G p -> Seq v G (p :-> q) -> Seq v G q
-| Reduct: forall (G:Ctx v)(p:P v),     Seq v (G;¬p) bot -> Seq v G p
+Inductive Seq (v:Type) (e:Eq v) : Ctx v -> P v -> Type :=
+| Extract:forall (G:Ctx v)(p:P v),      CtxVal G -> Fr p <= Fr' G -> Seq v e (G;p) p 
+| WeakenV:forall (G:Ctx v)(x:v)(p:P v), ~(x :: Fr' G) -> Seq v e G p -> Seq v e (G,x) p
+| WeakenP:forall (G:Ctx v)(p q:P v),    Fr q <= Fr' G -> Seq v e G p -> Seq v e (G;q) p
+| Deduct :forall (G:Ctx v)(p q:P v),    Seq v e (G;p) q -> Seq v e G (p :-> q)
+| Modus  :forall (G:Ctx v)(p q: P v),   Seq v e G p -> Seq v e G (p :-> q) -> Seq v e G q
+| Reduct :forall (G:Ctx v)(p:P v),      Seq v e (G;¬p) bot -> Seq v e G p
+| AxiomP :forall (G:Ctx v)(p:P v),      CtxVal G -> IsAxiom p -> Seq v e G p 
+| General:forall (G:Ctx v)(x:v)(p:P v), Seq v e (G,x) p -> Seq v e G (All x p) 
+| Special:forall (G:Ctx v)(x y:v)(p:P v),
+    CtxVal G              ->
+    Fr (All x p) <= Fr' G ->
+    ~ (y :: Fr' G)        -> 
+    Seq v e (G;All x p,y) (fmap (y <:> x) p)
 .
 
- 
+Arguments Seq     {v} {e}.
+Arguments Extract {v} {e}.
+Arguments WeakenV {v} {e}.
+Arguments WeakenP {v} {e}.
+Arguments Deduct  {v} {e}.
+Arguments Modus   {v} {e}.
+Arguments Reduct  {v} {e}.
+Arguments AxiomP  {v} {e}.
+Arguments General {v} {e}.
+Arguments Special {v} {e}.
+
+Notation "G :- p" := (Seq G p)
+  (at level 90, no associativity) : Fol2_Proof_scope.
+
+Open Scope Fol2_Proof_scope.
